Freigen/ExactCodensity.lean
@@ -5,9 +5,33 @@ namespace Freigen
 structure ExactCodensity (M : Type u → Type v) [Monad M] (α : Type _) where
   run : ∀ {β : Type u}, (α → M β) → M β
   exact : ∀ {β : Type u} (f : α → M β), run pure >>= f = run f
+  result : M α
+  result_eq : result = run pure
+
+@[ext]
+theorem ExactCodensity.ext
+    {M : Type u → Type v} [Monad M] {α : Type u}
+    {x y : ExactCodensity M α}
+    (h : ∀ {β : Type u} (f : α → M β), x.run f = y.run f) : x = y := by
+  cases x with
+  | mk xrun xexact xresult xresult_eq =>
+    cases y with
+    | mk yrun yexact yresult yresult_eq =>
+      have hrun : @xrun = @yrun := by
+        funext β f
+        exact h f
+      cases hrun
+      have : xresult = yresult := xresult_eq.trans yresult_eq.symm
+      cases this
+      rfl
 
 instance {M} [Monad M] [LawfulMonad M] : Monad (ExactCodensity M) where
-  pure a := ⟨fun f => f a, by simp⟩
+  pure a := {
+    run := fun f => f a
+    exact := by simp
+    result := pure a
+    result_eq := rfl
+  }
   bind x f := {
     run := fun g => x.run fun a => (f a).run g,
     exact := by
@@ -15,17 +39,31 @@ instance {M} [Monad M] [LawfulMonad M] : Monad (ExactCodensity M) where
       conv => lhs; rw [←x.exact]
       rw [bind_assoc]
       simp only [ExactCodensity.exact]
+    result := x.run fun a => (f a).result
+    result_eq := by
+      congr 1
+      funext a
+      exact (f a).result_eq
   }
 
 instance {M} [Monad M] [LawfulMonad M] : LawfulMonad (ExactCodensity M) := LawfulMonad.mk' _
-  (by intros; rfl)
-  (by intros; rfl)
-  (by intros; rfl)
+  (by intros; apply ExactCodensity.ext; intros; rfl)
+  (by intros; apply ExactCodensity.ext; intros; rfl)
+  (by intros; apply ExactCodensity.ext; intros; rfl)
 
 protected def ExactCodensity.equiv {M} [Monad M] [LawfulMonad M] {α : Type u} : ExactCodensity M α ≃ M α where
-  toFun x := x.run pure
-  invFun x := ⟨fun f => x >>= f, by simp⟩
-  left_inv x := by simp only [ExactCodensity.exact]
+  toFun x := x.result
+  invFun x := {
+    run := fun f => x >>= f
+    exact := by simp
+    result := x
+    result_eq := by simp
+  }
+  left_inv x := by
+    apply ExactCodensity.ext
+    intro β f
+    change x.result >>= f = x.run f
+    rw [x.result_eq, x.exact]
   right_inv x := by simp
 
 @[simp]
@@ -42,16 +80,27 @@ theorem ExactCodensity.equiv_bind
     (x : ExactCodensity M α)
     (f : α → ExactCodensity M β) :
     ExactCodensity.equiv (x >>= f) =
-      ExactCodensity.equiv x >>= fun a =>
+    ExactCodensity.equiv x >>= fun a =>
         ExactCodensity.equiv (f a) :=
-  (x.exact _).symm
+  by
+    change x.run (fun a => (f a).result) =
+      x.result >>= fun a => (f a).result
+    rw [x.result_eq, x.exact]
 
 def ExactCodensity.bind_def {M} [Monad M] [LawfulMonad M] {α β : Type _} (x : ExactCodensity M α) (f : α → ExactCodensity M β) :
-    x >>= f = ⟨fun g => x.run fun a => (f a).run g, by
-      intros
-      conv => lhs; rw [←x.exact]
-      rw [bind_assoc]
-      simp only [ExactCodensity.exact]⟩ := by
+    x >>= f = {
+      run := fun g => x.run fun a => (f a).run g
+      exact := by
+        intros
+        conv => lhs; rw [←x.exact]
+        rw [bind_assoc]
+        simp only [ExactCodensity.exact]
+      result := x.run fun a => (f a).result
+      result_eq := by
+        congr 1
+        funext a
+        exact (f a).result_eq
+    } := by
   rfl
 
 end Freigen
